proof/crefine/ARM/Interrupt_C.thy
@@ -27,7 +27,7 @@ lemma getIRQSlot_ccorres:
   "ccorres ((=) \<circ> Ptr) irqSlot_'
           \<top> UNIV hs
       (getIRQSlot irq)
-      (\<acute>irqSlot :== CTypesDefs.ptr_add \<acute>intStateIRQNode (sint (ucast (ucast irq ::word16) :: 32 signed word)))"
+      (\<acute>irqSlot :== CTypesDefs.ptr_add intStateIRQNode_Ptr (sint (ucast (ucast irq ::word16) :: 32 signed word)))"
   apply (rule ccorres_from_vcg[where P=\<top> and P'=UNIV])
   apply (rule allI, rule conseqPre, vcg)
   apply (clarsimp simp: getIRQSlot_def liftM_def getInterruptState_def
@@ -42,11 +42,11 @@ lemma getIRQSlot_ccorres:
 lemma ptr_add_assertion_irq_guard:
 "ccorres dc xfdc P Q hs a
      (Guard F
-       \<lbrace>uint irq = 0 \<or> array_assertion \<acute>intStateIRQNode (nat (uint irq)) (hrs_htd \<acute>t_hrs)\<rbrace>
+       \<lbrace>uint irq = 0 \<or> array_assertion intStateIRQNode_Ptr (nat (uint irq)) (hrs_htd \<acute>t_hrs)\<rbrace>
        c;;m)
   \<Longrightarrow> ccorres dc xfdc P Q hs a
             (Guard F
-              \<lbrace>ptr_add_assertion \<acute>intStateIRQNode
+              \<lbrace>ptr_add_assertion intStateIRQNode_Ptr
                 (sint (ucast (irq :: 16 word)::32 signed word)) False
                 (hrs_htd \<acute>t_hrs)\<rbrace> c ;; m)"
   by (simp add: ptr_add_assertion_def sint_ucast_eq_uint is_down)
@@ -71,10 +71,11 @@ proof -
     by (clarsimp)
   show ?thesis
   apply (cinit lift: irq_' slot_' cap_')
+   apply (rule ccorres_Guard_intStateIRQNode_array_Ptr)
    apply (rule ptr_add_assertion_irq_guard)
    apply (rule ccorres_move_array_assertion_irq)
-   apply (simp only:)
-   apply (ctac(no_vcg) add: getIRQSlot_ccorres)
+   apply (simp add: ucast_up_ucast is_up)
+   apply (ctac(no_vcg) add: getIRQSlot_ccorres[simplified])
      apply (rule ccorres_symb_exec_r)
        apply (ctac(no_vcg) add: cteDeleteOne_ccorres[where w="-1"])
         apply (ctac(no_vcg) add: cteInsert_ccorres)
@@ -106,10 +107,11 @@ lemma invokeIRQHandler_ClearIRQHandler_ccorres:
       (invokeIRQHandler (ClearIRQHandler irq))
       (Call invokeIRQHandler_ClearIRQHandler_'proc)"
   apply (cinit lift: irq_')
+   apply (rule ccorres_Guard_intStateIRQNode_array_Ptr)
    apply (rule ptr_add_assertion_irq_guard)
    apply (rule ccorres_move_array_assertion_irq)
-   apply (simp only: )
-   apply (ctac(no_vcg) add: getIRQSlot_ccorres)
+   apply (simp add: ucast_up_ucast is_up)
+   apply (ctac(no_vcg) add: getIRQSlot_ccorres[simplified])
      apply (rule ccorres_symb_exec_r)
        apply (ctac add: cteDeleteOne_ccorres[where w="-1"])
       apply vcg
